# Summary {.unnumbered}

## 4.4 Coordinate Systems

::: {#thm-4-8}

## Theorem 8

Let $\mathcal{B}=\left\{\mathbf{b}_1, \ldots, \mathbf{b}_n\right\}$ be a basis for a vector space $V$. Then the coordinate mapping $\mathbf{x} \mapsto[\mathbf{x}]_{\mathcal{B}}$ is a one-to-one linear transformation from $V$ onto $\mathbb{R}^n$.
:::

::: {.remark}

What this theorem means is that for a transformation $T: V \to \mathbb{R}^n$ which is defined as $\mathbf{x} \mapsto [\mathbf{x}]_{\mathcal{B}}$, $T$ is a linear transformation and is both one-to-one and onto.
:::

::: {#exr-4-4-p2}

## Practice Problem 2

The set $\mathcal{B}=\left\{1+t, 1+t^2, t+t^2\right\}$ is a basis for $\mathbb{P}_2$. Find the coordinate vector of $\mathbf{p}(t)=6+3 t-t^2$ relative to $\mathcal{B}$.
:::

::: {.remark}

One way to solve this is to equate the coefficients of the equation 
$$c_1(1+t) + c_2(1+t^2) + c_3(t+t^2)=6+3 t-t^2$$
and solve for $c_1,c_2,c_3$.

However, by observation, we can also first write $1+t,1+t^2,t+t^2,6+3t-t^2$ as $\begin{bmatrix}1\\ 1\\ 0\end{bmatrix}, \begin{bmatrix}1\\ 0\\ 1\end{bmatrix}, \begin{bmatrix}0\\ 1\\ 1\end{bmatrix}, \begin{bmatrix}6\\ 3\\ -1\end{bmatrix}$. Then, as for subspaces in $\mathbb{R}$, we solve the coefficients $\mathbf{c}$ using row reduction.
:::

::: {.callout-tip}

## Why does this method work?

Let $T: \mathbf{x} \mapsto [\mathbf{x}]_\mathcal{B}$, so $T$ is a bijective linear transformation.

\begin{align}
T(c_1\mathbf{b}_1 + \cdots + c_n\mathbf{b}_n) &= c_1 T(\mathbf{b}_1) + \cdots + c_n T(\mathbf{b}_n) \\
&= T(\mathbf{p})
\end{align}

where $T(\mathbf{b}_1),\dots,T(\mathbf{b}_n)$ are the coordinate vectors of the basis. Since $T$ is bijective, we can apply $T^{-1}$ to both side of the equation. Reversing the steps gives the same coefficients.

<!-- First, we formalize our original problem as follows: we aim to find the value of $T(\mathbf{p})$, where $T: \mathbf{p} \mapsto [\mathbf{p}]_\mathcal{B}$. If we knows $T_1: \mathbf{p} \mapsto [\mathbf{p}]_{\mathcal{B}'}$ and $T_2: [\mathbf{p}]_{\mathcal{B}'} \mapsto [\mathbf{p}]_{\mathcal{B}}$, then $T(\mathbf{p})=T_2(T_1(\mathbf{p}))$.

In our case, $\mathcal{B}'=\{1,t,t^2\}$, so $T_1$ is obvious. For each $\mathbf{b}_k \in \mathcal{B}$,

\begin{align}
T(\mathbf{b}_k)&=\mathbf{e}_k \\
&=T_2(T_2^{-1}(\mathbf{e}_k)) \\
&=T_2(T_2^{-1}([\mathbf{b}_k]_\mathcal{B})) \\
&=T_2([\mathbf{b}_k]_{\mathcal{B}'}) \\
&=T_2(T_1(\mathbf{b}_k))
\end{align}

Since $T,T_1,T_2$ are linear transformations, by proving that they yield the same result for each vector in their basis, we have shown that $T$ is equivalent to applying $T_1$ and then $T_2$. -->
:::

## Isomorphism

::: {.callout-tip}

## How to write rigorous solutions when using isomorphism?

In some problems, we are given
:::

## Solving for Bases Using Column Operations